SStructTT/SStruct/Runtime/Substitution.lean
@@ -1,112 +1,7 @@
 import SStructTT.SStruct.Runtime.Resolution
 
 namespace SStruct.Erasure
-namespace Runtime
-open Dynamic
 variable {Srt : Type} [ord : SrtOrder Srt]
-
-@[aesop safe (rule_sets := [subst]) [constructors]]
-inductive AgreeSubst :
-  (Var -> Tm Srt) -> (Var -> Tm Srt) -> Nat -> Ctx Srt -> Heap Srt -> Prop
-where
-  | nil {H σ σ'} :
-    WR H ->
-    HLower H ord.e ->
-    AgreeSubst σ σ' 0 [] H
-  | cons {Δ H σ σ' A x r s} :
-    AgreeSubst σ σ' x Δ H ->
-    AgreeSubst (up σ) (up σ') (x + 1) (A :⟨r, s⟩ Δ) H
-  | intro_im {Δ H σ σ' A m m' s} :
-    AgreeSubst σ σ' 0 Δ H ->
-    AgreeSubst (m .: σ) (m' .: σ') 0 (A :⟨.im, s⟩ Δ) H
-  | intro_ex {Δ H1 H2 H3 σ σ' m m' A s} :
-    WR H2 ->
-    HLower H2 s ->
-    HMerge H1 H2 H3 ->
-    H2 ⊢ m ▷ m' ->
-    AgreeSubst σ σ' 0 Δ H1 ->
-    AgreeSubst (m .: σ) (m' .: σ') 0 (A :⟨.ex, s⟩ Δ) H3
-
-lemma AgreeSubst.implicit_image {Δ : Ctx Srt} {H σ σ' x} :
-    AgreeSubst σ σ' x Δ H -> Implicit Δ -> HLower H ord.e := by
-  intro agr im; induction agr
-  case nil => assumption
-  case cons ih =>
-    simp at im; replace ⟨e, im⟩ := im; subst_vars
-    apply ih; apply im
-  case intro_im ih =>
-    simp at im
-    apply ih; apply im
-  case intro_ex => simp at im
-
-lemma AgreeSubst.lower_image {Δ : Ctx Srt} {H σ σ' x s} :
-    AgreeSubst σ σ' x Δ H -> Lower Δ s -> HLower H s := by
-  intro agr lw; induction agr generalizing s
-  case nil hw =>
-    apply hw.weaken (ord.e_min _)
-  case cons => cases lw <;> aesop
-  case intro_im => cases lw; aesop
-  case intro_ex wr hw2 mrg erm agr ih =>
-    cases lw; case ex le lw =>
-    have hw1 := ih lw
-    replace hw2 := hw2.weaken le
-    apply mrg.lower_image hw1 hw2
-
-lemma AgreeSubst.ids {Δ : Ctx Srt} {H x} :
-    WR H -> HLower H ord.e -> x = Δ.length -> AgreeSubst ids ids x Δ H := by
-  intro wr lw e; subst e
-  induction Δ
-  case nil => constructor <;> assumption
-  case cons hd tl ih =>
-    simp; have ⟨A, r, s⟩ := hd
-    replace ih := ih.cons (A := A) (r := r) (s := s)
-    asimp at ih; apply ih
-
-lemma AgreeSubst.subst_var {Δ : Ctx Srt} {H σ σ' i x} :
-    AgreeSubst σ σ' i Δ H -> x < i -> .var x = σ x := by
-  intro agr le; induction agr generalizing x
-  all_goals try trivial
-  case cons i _ _  agr ih =>
-    cases x with
-    | zero => asimp
-    | succ x =>
-      simp at le; asimp
-      have e := ih le
-      rw[<-e]; asimp
-
-lemma AgreeSubst.nf_subst {Δ : Ctx Srt} {H σ σ' i x m} :
-    AgreeSubst σ σ' i Δ H -> NF x m -> x ≤ i -> m = m.[σ] := by
-  intro agr nf lw; induction m generalizing Δ H σ σ' i x
-  all_goals simp_all
-  case var =>
-    asimp; apply agr.subst_var
-    apply nf.trans_le lw
-  case lam ih =>
-    asimp; apply ih
-    . apply AgreeSubst.cons agr
-      constructor; apply 0; constructor; apply ord.e
-    . assumption
-    . simp[lw]
-  case prj ihm ihn =>
-    have ⟨nf1, nf2⟩ := nf
-    asimp; split_ands
-    . aesop
-    . apply ihn
-      . apply AgreeSubst.cons
-        constructor; apply 0; constructor; apply ord.e
-        apply AgreeSubst.cons
-        constructor; apply 0; constructor; apply ord.e
-        apply agr
-      . aesop
-      . simp[lw]
-  all_goals asimp; try aesop
-
-lemma AgreeSubst.wr_heap {Δ : Ctx Srt} {H σ σ' i} :
-    AgreeSubst σ σ' i Δ H -> WR H := by
-  intro agr; induction agr
-  all_goals try aesop
-  case intro_ex wr2 _ mrg _ _ wr1 =>
-    apply mrg.merge_wr wr1 wr2
 
 def IdRename (i : Var) (ξ : Var -> Var) : Prop := ∀ x, x < i -> ξ x = x
 
@@ -149,10 +44,104 @@ lemma NF.id_rename {m : Tm Srt} {i ξ} :
     have ⟨nf1, nf2⟩ := nf
     asimp; aesop
 
+namespace Runtime
+open Dynamic
+
+@[aesop safe (rule_sets := [subst]) [constructors]]
+inductive AgreeSubst :
+  (Var -> Tm Srt) -> (Var -> Tm Srt) -> Nat -> Ctx Srt -> Heap Srt -> Prop
+where
+  | nil {σ σ'} :
+    AgreeSubst σ σ' 0 [] ∅
+  | cons {Δ H σ σ' A x r s} :
+    AgreeSubst σ σ' x Δ H ->
+    AgreeSubst (up σ) (up σ') (x + 1) (A :⟨r, s⟩ Δ) H
+  | intro_im {Δ H σ σ' A m m' s} :
+    AgreeSubst σ σ' 0 Δ H ->
+    AgreeSubst (m .: σ) (m' .: σ') 0 (A :⟨.im, s⟩ Δ) H
+  | intro_ex {Δ H1 H2 H3 σ σ' m m' A s} :
+    WR H2 ->
+    HLower H2 s ->
+    HMerge H1 H2 H3 ->
+    H2 ⊢ m ▷ m' ->
+    AgreeSubst σ σ' 0 Δ H1 ->
+    AgreeSubst (m .: σ) (m' .: σ') 0 (A :⟨.ex, s⟩ Δ) H3
+
+lemma AgreeSubst.implicit_image {Δ : Ctx Srt} {H σ σ' x} :
+    AgreeSubst σ σ' x Δ H -> Implicit Δ -> H = ∅ := by
+  intro agr im; induction agr
+  case nil => rfl
+  case cons ih =>
+    simp at im; replace ⟨e, im⟩ := im; subst_vars
+    apply ih; apply im
+  case intro_im ih =>
+    simp at im
+    apply ih; apply im
+  case intro_ex => simp at im
+
+lemma AgreeSubst.lower_image {Δ : Ctx Srt} {H σ σ' x s} :
+    AgreeSubst σ σ' x Δ H -> Lower Δ s -> HLower H s := by
+  intro agr lw; induction agr generalizing s
+  case nil => apply HLower.empty
+  case cons => cases lw <;> aesop
+  case intro_im => cases lw; aesop
+  case intro_ex wr hw2 mrg erm agr ih =>
+    cases lw; case ex le lw =>
+    have hw1 := ih lw
+    replace hw2 := hw2.weaken le
+    apply mrg.lower_image hw1 hw2
+
+lemma AgreeSubst.subst_var {Δ : Ctx Srt} {H σ σ' i x} :
+    AgreeSubst σ σ' i Δ H -> x < i -> .var x = σ' x := by
+  intro agr le; induction agr generalizing x
+  all_goals try trivial
+  case cons i _ _  agr ih =>
+    cases x with
+    | zero => asimp
+    | succ x =>
+      simp at le; asimp
+      have e := ih le
+      rw[<-e]; asimp
+
+lemma AgreeSubst.nf_subst {Δ : Ctx Srt} {H σ σ' i x m} :
+    AgreeSubst σ σ' i Δ H -> NF x m -> x ≤ i -> m = m.[σ'] := by
+  intro agr nf lw; induction m generalizing Δ H σ σ' i x
+  all_goals simp_all
+  case var =>
+    asimp; apply agr.subst_var
+    apply nf.trans_le lw
+  case lam ih =>
+    asimp; apply ih
+    . apply AgreeSubst.cons agr
+      constructor; apply 0; constructor; apply ord.e
+    . assumption
+    . simp[lw]
+  case prj ihm ihn =>
+    have ⟨nf1, nf2⟩ := nf
+    asimp; split_ands
+    . aesop
+    . apply ihn
+      . apply AgreeSubst.cons
+        constructor; apply 0; constructor; apply ord.e
+        apply AgreeSubst.cons
+        constructor; apply 0; constructor; apply ord.e
+        apply agr
+      . aesop
+      . simp[lw]
+  all_goals asimp; try aesop
+
+lemma AgreeSubst.wr_heap {Δ : Ctx Srt} {H σ σ' i} :
+    AgreeSubst σ σ' i Δ H -> WR H := by
+  intro agr; induction agr
+  all_goals try aesop
+  case nil => apply WR.empty
+  case intro_ex wr2 _ mrg _ _ wr1 =>
+    apply mrg.merge_wr wr1 wr2
+
 lemma Resolve.id_rename {H : Heap Srt} {m m' i ξ} :
     H ⊢ m ▷ m' -> WR H -> IdRename i ξ -> H ⊢ m.[ren ξ] ▷ m'.[ren ξ] := by
   intro rs wr idr; induction rs generalizing i ξ
-  case var => asimp; constructor; aesop
+  case var => asimp; constructor
   case lam lw _ ih =>
     asimp; apply Resolve.lam lw
     replace ih := ih wr idr.up
@@ -172,8 +161,8 @@ lemma Resolve.id_rename {H : Heap Srt} {m m' i ξ} :
     replace ihm := ihm wr1 idr
     replace ihn := ihn wr2 idr.up.up; asimp at ihn
     asimp; apply Resolve.prj mrg ihm ihn
-  case tt => asimp; constructor; assumption
-  case ff => asimp; constructor; assumption
+  case tt => asimp; constructor
+  case ff => asimp; constructor
   case ite mrg rsm rsn1 rsn2 ihm ihn1 ihn2 =>
     have ⟨wr1, wr2⟩ := mrg.split_wr wr
     replace ihm := ihm wr1 idr
@@ -185,11 +174,11 @@ lemma Resolve.id_rename {H : Heap Srt} {m m' i ξ} :
     replace ihm := ihm wr1 idr
     replace ihn := ihn wr2 idr
     asimp; apply Resolve.drop mrg lw mem ihm ihn
-  case ptr lk erm ihm =>
+  case ptr l m n s h rsm ihm =>
     asimp
-    have nfm := lk.nf wr
-    have wr' := lk.wr_image wr
-    have nfm' := (erm.nf_image wr' nfm).weaken (zero_le i)
+    have wr0 := wr.erase l; simp[Heap.erase_insert,h] at wr0
+    have nfm' := rsm.nf_image wr0 (wr.nf l m s (by simp))
+    have nfm' := nfm'.weaken (zero_le i)
     rw[<-nfm'.id_rename idr]
     constructor <;> assumption
   case null => asimp; constructor; assumption
@@ -201,8 +190,8 @@ lemma AgreeSubst.has {Δ : Ctx Srt} {H σ σ' x i s A} :
   case cons agr ih =>
     cases hs
     case nil im =>
-      have lw := agr.implicit_image im
-      asimp; constructor; assumption
+      rw[agr.implicit_image im]
+      asimp; constructor
     case cons =>
       asimp; apply Resolve.id_rename
       . aesop
@@ -213,8 +202,9 @@ lemma AgreeSubst.has {Δ : Ctx Srt} {H σ σ' x i s A} :
   case intro_ex wr lw mrg rsm agr ih =>
     cases hs; case nil im =>
     asimp
-    have lw := agr.implicit_image im
-    apply rsm.weaken_merge mrg.sym lw
+    rw[agr.implicit_image im] at mrg
+    have e := mrg.sym.empty_inv; subst e
+    assumption
 
 lemma AgreeSubst.split {Δ1 Δ2 Δ3 : Ctx Srt} {H3 σ σ' x} :
     AgreeSubst σ σ' x Δ3 H3 -> Merge Δ1 Δ2 Δ3 ->
@@ -223,14 +213,12 @@ lemma AgreeSubst.split {Δ1 Δ2 Δ3 : Ctx Srt} {H3 σ σ' x} :
       AgreeSubst σ σ' x Δ1 H1 ∧
       AgreeSubst σ σ' x Δ2 H2 := by
   intro agr mrg; induction agr generalizing Δ1 Δ2
-  case nil wr lw =>
+  case nil =>
     cases mrg
-    have ⟨H1, H2, lw1, lw2, mrg⟩ := lw.split_lower ord.e_contra
-    have ⟨wr1, wr2⟩ := mrg.split_wr wr
-    exists H1, H2; and_intros
-    . assumption
-    . constructor <;> assumption
-    . constructor <;> assumption
+    exists ∅, ∅; and_intros
+    . apply HMerge.empty
+    . constructor
+    . constructor
   case cons agr ih =>
     cases mrg
     case contra mrg =>
@@ -299,12 +287,12 @@ lemma Resolved.substitution {H1 H2 H3 : Heap Srt} {Γ Δ m n n' A σ σ' x} :
     asimp; cases rs
     case var lw =>
       asimp
-      apply Resolve.weaken_merge mrg.sym lw
+      have e := mrg.sym.empty_inv; subst_vars
       apply agr.has hs
-    case ptr lk rsm =>
+    case ptr l m s h rsm =>
       cases rsm
-      case var => exfalso; apply lk.not_wr_var wr
-      case ptr => exfalso; apply lk.not_wr_ptr wr
+      case var => have wr := wr l; simp at wr
+      case ptr => have wr := wr l; simp at wr
   case lam_im Δ A B m m' s sA iA lw tyA erm ihm =>
     have lw2 := agr.lower_image lw
     asimp; cases rs
@@ -313,19 +301,25 @@ lemma Resolved.substitution {H1 H2 H3 : Heap Srt} {Γ Δ m n n' A σ σ' x} :
       have lw3 := mrg.lower_image lw1 lw2
       replace ihm := ihm erm wr mrg agr.cons
       apply Resolve.lam lw3 ihm
-    case ptr lk rsm =>
+    case ptr l x s h rsm =>
       cases rsm
-      case lam erm lw1 =>
+      case lam rsm _ =>
         asimp
-        have nf := lk.nf wr; simp at nf
-        have wr := lk.wr_image wr
-        have ⟨H3, lk, mrg⟩ := lk.merge mrg
-        apply Resolve.ptr lk
-        apply Resolve.lam (mrg.lower_image lw1 lw2)
-        have agr : AgreeSubst (up σ) (up σ') (x + 1) (A :⟨.im, sA⟩ Δ) H2 := by
+        have nf0 := wr l; simp at nf0
+        replace ⟨nf0, e⟩ := nf0; subst e
+        have wr0 := wr.erase l; simp[Heap.erase_insert,h] at wr0
+        have nf1 := rsm.nf_image wr0 nf0
+        have nf2 : NF 0 (.lam m' s) := by simp; assumption
+        have erm := Erased.lam_im lw tyA erm
+        have im := (erm.nf_stack nf2).toImplicit
+        have e := agr.implicit_image im; subst e
+        have e := mrg.empty_inv; subst e
+        have agr : AgreeSubst (up σ) (up σ') (x + 1) (A :⟨.im, sA⟩ Δ) ∅ := by
           apply AgreeSubst.cons; assumption
-        rw[agr.nf_subst nf (by simp)]; aesop
-      case ptr => exfalso; apply lk.not_wr_ptr wr
+        rw[<-agr.nf_subst nf1 (by simp)]
+        apply Resolve.ptr h
+        constructor <;> assumption
+      case ptr => have wr := wr l; simp at wr
   case lam_ex Δ A B m m' s sA iA lw tyA erm ihm =>
     have lw2 := agr.lower_image lw
     asimp; cases rs
@@ -334,19 +328,25 @@ lemma Resolved.substitution {H1 H2 H3 : Heap Srt} {Γ Δ m n n' A σ σ' x} :
       have lw3 := mrg.lower_image lw1 lw2
       replace ihm := ihm erm wr mrg agr.cons
       apply Resolve.lam lw3 ihm
-    case ptr lk rsm =>
+    case ptr l x s h rsm =>
       cases rsm
-      case lam erm lw1 =>
+      case lam rsm _ =>
         asimp
-        have nf := lk.nf wr; simp at nf
-        have wr := lk.wr_image wr
-        have ⟨H3, lk, mrg⟩ := lk.merge mrg
-        apply Resolve.ptr lk
-        apply Resolve.lam (mrg.lower_image lw1 lw2)
-        have agr : AgreeSubst (up σ) (up σ') (x + 1) (A :⟨.ex, sA⟩ Δ) H2 := by
+        have nf0 := wr l; simp at nf0
+        replace ⟨nf0, e⟩ := nf0; subst e
+        have wr0 := wr.erase l; simp[Heap.erase_insert,h] at wr0
+        have nf1 := rsm.nf_image wr0 nf0
+        have nf2 : NF 0 (.lam m' s) := by simp; assumption
+        have erm := Erased.lam_ex lw tyA erm
+        have im := (erm.nf_stack nf2).toImplicit
+        have e := agr.implicit_image im; subst e
+        have e := mrg.empty_inv; subst e
+        have agr : AgreeSubst (up σ) (up σ') (x + 1) (A :⟨.im, sA⟩ Δ) ∅ := by
           apply AgreeSubst.cons; assumption
-        rw[agr.nf_subst nf (by simp)]; aesop
-      case ptr => exfalso; apply lk.not_wr_ptr wr
+        rw[<-agr.nf_subst nf1 (by simp)]
+        apply Resolve.ptr h
+        constructor <;> assumption
+      case ptr => have wr := wr l; simp at wr
   case app_im A B m m' n s erm tyn ihm =>
     asimp; cases rs
     case app mrg1 rsm rsn =>
@@ -356,10 +356,10 @@ lemma Resolved.substitution {H1 H2 H3 : Heap Srt} {Γ Δ m n n' A σ σ' x} :
       asimp; apply Resolve.app mrg'
       . apply ihm rsm wr1 mrg2 agr
       . assumption
-    case ptr lk rsm =>
+    case ptr l _ _ _ rsm =>
       cases rsm
-      case app => have vl := lk.wr_value wr; cases vl
-      case ptr => exfalso; apply lk.not_wr_ptr wr
+      case app => have wr := wr l; simp at wr
+      case ptr => have wr := wr l; simp at wr
   case app_ex mrg0 erm ern ihm ihn =>
     asimp; cases rs
     case app mrg1 rsm rsn =>
@@ -369,10 +369,10 @@ lemma Resolved.substitution {H1 H2 H3 : Heap Srt} {Γ Δ m n n' A σ σ' x} :
       replace ihm := ihm rsm wr1 mrg1' agr1
       replace ihn := ihn rsn wr2 mrg2' agr2
       asimp; apply Resolve.app mrg3 ihm ihn
-    case ptr lk rsm =>
+    case ptr l _ _ _ rsm =>
       cases rsm
-      case app => have vl := lk.wr_value wr; cases vl
-      case ptr => exfalso; apply lk.not_wr_ptr wr
+      case app => have wr := wr l; simp at wr
+      case ptr => have wr := wr l; simp at wr
   case tup_im ty erm tyn ihm =>
     asimp; cases rs
     case tup mrg1 rsm rsn =>
@@ -382,22 +382,21 @@ lemma Resolved.substitution {H1 H2 H3 : Heap Srt} {Γ Δ m n n' A σ σ' x} :
       asimp; apply Resolve.tup mrg'
       . apply ihm rsm wr1 mrg2 agr
       . assumption
-    case ptr lk rsm =>
-      cases rsm
-      case tup mrg1 rsm1 rsm2 =>
-        asimp
-        have nf := lk.nf wr; simp at nf; have ⟨nf1, nf2⟩ := nf
-        have wr := lk.wr_image wr
-        have ⟨wr1, wr2⟩ := mrg1.split_wr wr
-        have ⟨lw2, e⟩ := rsm2.null_inv wr2; subst e
-        have ⟨H3', lk', mrg3'⟩ := lk.merge mrg
-        have ⟨H2', mrg2', mrg3'⟩ := mrg3'.split mrg1
-        apply Resolve.ptr lk'
-        apply Resolve.tup mrg3'
-        . rw[agr.nf_subst nf1 (by simp)]
-          apply ihm rsm1 wr1 mrg2' agr
-        . assumption
-      case ptr => exfalso; apply lk.not_wr_ptr wr
+    case ptr l _ _ h rsm =>
+      asimp; cases rsm
+      case tup mrg0 rsm rsn =>
+        have wr0 := wr.erase l; simp[Heap.erase_insert,h] at wr0
+        have ⟨wr1, wr2⟩ := mrg0.split_wr wr0
+        have nf0 := wr.nf l; simp at nf0
+        rcases nf0 with ⟨nf1, nf2⟩
+        have nf1' := rsm.nf_image wr1 nf1
+        have im := (erm.nf_stack nf1').toImplicit
+        have e := agr.implicit_image im; subst e
+        have e := mrg.empty_inv; subst e
+        rw[<-agr.nf_subst nf1' (by simp)]
+        apply Resolve.ptr h
+        constructor <;> assumption
+      case ptr => have wr := wr l; simp at wr
   case tup_ex mrg0 ty erm ern ihm ihn =>
     asimp; cases rs
     case tup mrg1 rsm rsn =>
@@ -407,22 +406,25 @@ lemma Resolved.substitution {H1 H2 H3 : Heap Srt} {Γ Δ m n n' A σ σ' x} :
       replace ihm := ihm rsm wr1 mrg1' agr1
       replace ihn := ihn rsn wr2 mrg2' agr2
       asimp; apply Resolve.tup mrg3 ihm ihn
-    case ptr lk rsm =>
-      cases rsm
-      case tup mrg1 rsm1 rsm2 =>
-        asimp
-        have nf := lk.nf wr; simp at nf; have ⟨nf1, nf2⟩ := nf
-        have ⟨H3', lk', mrg'⟩ := lk.merge mrg
-        have ⟨Ha, Hb, mrg2, agr1, agr2⟩ := agr.split mrg0
-        have ⟨H1', H2', mrg3', mrg1', mrg2'⟩ := mrg'.distr mrg1 mrg2
-        have ⟨wr1, wr2⟩ := mrg1.split_wr (lk.wr_image wr)
-        apply Resolve.ptr lk'
-        apply Resolve.tup mrg3'
-        . rw[agr.nf_subst nf1 (by simp)]
-          apply ihm rsm1 wr1 mrg1' agr1
-        . rw[agr.nf_subst nf2 (by simp)]
-          apply ihn rsm2 wr2 mrg2' agr2
-      case ptr => exfalso; apply lk.not_wr_ptr wr
+    case ptr l _ _ h rsm =>
+      asimp; cases rsm
+      case tup mrg1 rsm rsn =>
+        have wr0 := wr.erase l; simp[Heap.erase_insert,h] at wr0
+        have ⟨wr1, wr2⟩ := mrg1.split_wr wr0
+        have nf0 := wr.nf l; simp at nf0
+        rcases nf0 with ⟨nf1, nf2⟩
+        have nf1' := rsm.nf_image wr1 nf1
+        have nf2' := rsn.nf_image wr2 nf2
+        have im1 := (erm.nf_stack nf1').toImplicit
+        have im2 := (ern.nf_stack nf2').toImplicit
+        have im := mrg0.implicit_image im1 im2
+        have e := agr.implicit_image im; subst e
+        have e := mrg.empty_inv; subst e
+        rw[<-agr.nf_subst nf1' (by simp)]
+        rw[<-agr.nf_subst nf2' (by simp)]
+        apply Resolve.ptr h
+        constructor <;> assumption
+      case ptr => have wr := wr l; simp at wr
   case prj_im mrg0 tyC erm ern ihm ihn =>
     asimp; cases rs
     case prj mrg1 rsm rsn =>
@@ -432,10 +434,10 @@ lemma Resolved.substitution {H1 H2 H3 : Heap Srt} {Γ Δ m n n' A σ σ' x} :
       replace ihm := ihm rsm wr1 mrg1' agr1
       replace ihn := ihn rsn wr2 mrg2' agr2.cons.cons
       asimp; apply Resolve.prj mrg3 ihm ihn
-    case ptr lk rsm =>
-      cases rsm
-      case prj => have vl := lk.wr_value wr; cases vl
-      case ptr => exfalso; apply lk.not_wr_ptr wr
+    case ptr l _ _ h rsm =>
+      asimp; cases rsm
+      case prj => have wr := wr l; simp at wr
+      case ptr => have wr := wr l; simp at wr
   case prj_ex mrg0 tyC erm ern ihm ihn =>
     asimp; cases rs
     case prj mrg1 rsm rsn =>
@@ -445,34 +447,32 @@ lemma Resolved.substitution {H1 H2 H3 : Heap Srt} {Γ Δ m n n' A σ σ' x} :
       replace ihm := ihm rsm wr1 mrg1' agr1
       replace ihn := ihn rsn wr2 mrg2' agr2.cons.cons
       asimp; apply Resolve.prj mrg3 ihm ihn
-    case ptr lk rsm =>
-      cases rsm
-      case prj => have vl := lk.wr_value wr; cases vl
-      case ptr => exfalso; apply lk.not_wr_ptr wr
+    case ptr l _ _ h rsm =>
+      asimp; cases rsm
+      case prj => have wr := wr l; simp at wr
+      case ptr => have wr := wr l; simp at wr
   case tt im =>
-    have lw2 := agr.implicit_image im
+    have e := agr.implicit_image im; subst e
+    have e := mrg.empty_inv; subst e
     asimp; cases rs
-    case tt lw1 =>
-      asimp; apply Resolve.tt (mrg.lower_image lw1 lw2)
-    case ptr lk rsm =>
+    case tt => asimp; apply Resolve.tt
+    case ptr l _ _ h rsm =>
       cases rsm
-      case tt lw1 =>
-        have ⟨H3', lk', mrg'⟩ := lk.merge mrg
-        asimp; apply Resolve.ptr lk'
-        apply Resolve.tt (mrg'.lower_image lw1 lw2)
-      case ptr => exfalso; apply lk.not_wr_ptr wr
+      case tt =>
+        asimp; apply Resolve.ptr h
+        constructor
+      case ptr => have wr := wr l; simp at wr
   case ff im =>
-    have lw2 := agr.implicit_image im
+    have e := agr.implicit_image im; subst e
+    have e := mrg.empty_inv; subst e
     asimp; cases rs
-    case ff lw1 =>
-      asimp; apply Resolve.ff (mrg.lower_image lw1 lw2)
-    case ptr lk rsm =>
+    case ff => asimp; apply Resolve.ff
+    case ptr l _ _ h rsm =>
       cases rsm
-      case ff lw1 =>
-        have ⟨H3', lk', mrg'⟩ := lk.merge mrg
-        asimp; apply Resolve.ptr lk'
-        apply Resolve.ff (mrg'.lower_image lw1 lw2)
-      case ptr => exfalso; apply lk.not_wr_ptr wr
+      case ff =>
+        asimp; apply Resolve.ptr h
+        constructor
+      case ptr => have wr := wr l; simp at wr
   case ite mrg0 tyA erm ern1 ern2 ihm ihn1 ihn2 =>
     asimp; cases rs
     case ite mrg1 rsm rsn1 rsn2 =>
@@ -483,10 +483,10 @@ lemma Resolved.substitution {H1 H2 H3 : Heap Srt} {Γ Δ m n n' A σ σ' x} :
       replace ihn1 := ihn1 rsn1 wr2 mrg2' agr2
       replace ihn2 := ihn2 rsn2 wr2 mrg2' agr2
       asimp; apply Resolve.ite mrg3 ihm ihn1 ihn2
-    case ptr lk rsm =>
+    case ptr l _ _ h rsm =>
       cases rsm
-      case ite => have vl := lk.wr_value wr; cases vl
-      case ptr => exfalso; apply lk.not_wr_ptr wr
+      case ite => have wr := wr l; simp at wr
+      case ptr => have wr := wr l; simp at wr
   case rw ih => aesop
   case drop mrg0 lw0 h0 _ _ ihm ihn =>
     asimp; cases rs
@@ -502,10 +502,10 @@ lemma Resolved.substitution {H1 H2 H3 : Heap Srt} {Γ Δ m n n' A σ σ' x} :
       replace ihm := ihm rsm wr1 mrg1' agr1
       replace ihn := ihn rsn wr2 mrg2' agr2
       asimp; apply Resolve.drop mrg3 lw h0 ihm ihn
-    case ptr lk rsm =>
-      cases rsm
-      case drop => have vl := lk.wr_value wr; cases vl
-      case ptr => exfalso; apply lk.not_wr_ptr wr
+    case ptr l _ _ h rsm =>
+      asimp; cases rsm
+      case drop => have wr := wr l; simp at wr
+      case ptr => have wr := wr l; simp at wr
   case conv => aesop
 
 lemma Resolved.subst_im {H : Heap Srt} {m n n' A B s} :
@@ -514,7 +514,7 @@ lemma Resolved.subst_im {H : Heap Srt} {m n n' A B s} :
   intro rsm
   apply rsm.substitution HMerge.empty
   apply AgreeSubst.intro_im
-  apply AgreeSubst.ids WR.empty HLower.empty (by simp)
+  constructor
 
 lemma Resolved.subst_ex {H1 H2 H3 : Heap Srt} {m n n' t t' A B s} :
     WR H2 -> HLower H2 s -> HMerge H1 H2 H3 ->
@@ -525,4 +525,4 @@ lemma Resolved.subst_ex {H1 H2 H3 : Heap Srt} {m n n' t t' A B s} :
   apply rsm.substitution mrg
   apply AgreeSubst.intro_ex wr lw HMerge.empty.sym
   . assumption
-  . apply AgreeSubst.ids WR.empty HLower.empty (by simp)
+  . constructor
